Add lemmata

prim_rec.lean
@@ -23,17 +23,32 @@ def eval : forall {k}, prim_rec k -> (fin k -> nat) -> nat
   let ⟨x, y⟩ := fin_seq.pop arg in
   h x y
 
-lemma zero.is_zero: eval zero fin_seq.empty = 0 :=
+@[simp] lemma zero.is_zero: eval zero fin_seq.empty = 0 :=
 begin
   reflexivity,
 end
 
-lemma succ.is_succ: forall x, eval prim_rec.succ (fun _, x) = x + 1 :=
+def const: nat -> prim_rec 0
+| 0 := zero
+| (k + 1) := comp succ ({const k}: fin_seq _ _) 
+
+@[simp] def const.is_const: forall x, eval (const x) fin_seq.empty = x :=
+begin
+  intro x,
+  induction x with x' ih,
+  { reflexivity },
+  {
+    simp [eval, const],
+    rw ih,
+  },
+end
+
+@[simp] lemma succ.is_succ: forall x, eval prim_rec.succ ({x}: fin_seq _ _) = x + 1 :=
 fun x,
 calc
-  eval prim_rec.succ (fun _, x) = x + 1 : by unfold eval; reflexivity
+  eval prim_rec.succ ({x}: fin_seq _ _) = x + 1 : by unfold eval; reflexivity
 
-lemma uncurry_1: forall v: nat, fin_seq.pop (fun _: fin 1, v) = ⟨v, fin_seq.empty⟩ :=
+lemma uncurry_1: forall v: nat, fin_seq.pop {v} = ⟨v, fin_seq.empty⟩ :=
   fin_seq.pop_1
 
 lemma curry_at_0: forall k v (rest: fin k -> nat), fin_seq.push v rest 0 = v :=
@@ -49,24 +64,86 @@ end
 
 
 def id: prim_rec 1 := prim_rec.prec prim_rec.zero
-  (prim_rec.comp prim_rec.succ (fun _, prim_rec.proj 0))
+  (prim_rec.comp prim_rec.succ ({prim_rec.proj 0}: fin_seq _ _))
 
-
-lemma id.is_id : forall x, eval id (fun _, x) = x :=
+@[simp] lemma id.is_id : forall x, eval id ({x}: fin_seq 1 nat) = x :=
 begin
   intro x,
   induction x with x' ih,
   reflexivity,
-  show eval id
-      (fun _ : fin 1, x' + 1) =
+  show eval id ({x' + 1}: fin_seq _ _) =
     x' + 1,
   calc
-    eval id
-      (fun _ : fin 1, x' + 1)
-    = eval id
-      (fun _ : fin 1, x') + 1 : by reflexivity
+    eval id ({x' + 1}: fin_seq _ _)
+    = eval id ({x'}: fin_seq _ _) + 1 : by reflexivity
 ... = x' + 1 :
       by rw ih
+end
+
+def pred: prim_rec 1 := prec zero (proj 1)
+
+@[simp] lemma pred.is_pred: forall x, eval pred ({x}: fin_seq _ _) = x - 1 :=
+begin
+  intro x,
+  cases x with x',
+  { reflexivity },
+  { reflexivity },
+end
+
+def is_zero: prim_rec 1 := prec (const 1) (comp zero (fun _, proj 0))
+
+@[simp] lemma is_zero.is_is_zero: forall x, eval is_zero ({x}: fin_seq 1 nat) = if decidable.to_bool (x = 0) then 1 else 0 :=
+begin
+  intro x,
+  cases x with x',
+  { reflexivity },
+  { reflexivity },
+end
+
+-- S(x) + y = S(x + y)
+def add: prim_rec 2 := prec id (comp succ ({proj 0}: fin_seq _ _))
+-- sub_rev(x, y) = y - x
+def sub_rev: prim_rec 2 := prec id (comp pred ({proj 0}: fin_seq _ _))
+def sub: prim_rec 2 := comp sub_rev (fin_seq.push (proj 1) {proj 0})
+def mul: prim_rec 2 := prec (comp zero (fun _, succ)) (comp add (fin_seq.push (proj 1) {proj 2}))
+
+@[simp] lemma add.is_add: forall x y, eval add (fin_seq.push x {y}) = x + y :=
+begin
+  intro x,
+  induction x with x' ih,
+  {
+    intro y,
+    rw nat.add_comm,
+    rw nat.add_zero,
+    simp [add, eval],
+    reflexivity,
+  },
+  {
+    intro y,
+    change add.eval (fin_seq.push x' {y}) + 1 = x'.succ + y,
+    rw ih,
+    rw nat.add_comm x'.succ y,
+    rw nat.add_succ y x',
+    rw nat.add_comm y x',
+  },
+end
+
+@[simp] lemma sub_rev.is_sub_rev: forall x y, eval sub_rev (fin_seq.push x {y}) = y - x :=
+begin
+  intro x,
+  induction x with x' ih,
+  {
+    intro y,
+    simp [sub_rev, eval],
+    reflexivity,
+  },
+  {
+    intro y,
+    change pred.eval ({sub_rev.eval (fin_seq.push x' {y})}: fin_seq _ _) = y - x'.succ,
+    simp,
+    rw ih,
+    reflexivity,
+  },
 end
 
 end prim_rec
